Examples/ApproxMC.lean
@@ -1,0 +1,17 @@
+import LeanSAT
+
+open LeanSAT
+
+instance : Solver IO := Solver.Impl.DimacsCommand "cadical"
+instance : Solver.ApproxModelCount IO := Solver.Impl.ApproxMCCommand
+
+def main : IO Unit := do
+  let formula : Formula :=
+    (0 ∨ 1 ∨ 2) ∧ ¬0
+  IO.println formula.vars
+  let res ← Solver.solve formula
+  IO.println res
+  let res ← Solver.ApproxModelCount.approxModelCount formula formula.vars
+  IO.println res
+
+#eval main
