LeanSAT.lean
@@ -1,6 +1,5 @@
 import LeanSAT.AuxDefs
 import LeanSAT.CNF
 import LeanSAT.Constraint
-import LeanSAT.Dimacs
 import LeanSAT.EncCNF
 import LeanSAT.Solver
