LeanSAT/Solver/Basic.lean
@@ -1,0 +1,57 @@
+import Std.Data.HashMap
+import LeanSAT.CNF
+
+open Std
+
+namespace LeanSAT.Solver
+
+inductive Res
+| sat (assn : Assn)
+| unsat
+| error
+
+instance : ToString Res where
+  toString  | .error => "error"
+            | .unsat => "unsat"
+            | .sat assn => "sat: " ++ toString assn
+
+def Res.isSat : Res → Bool
+| .sat _  => true
+| _       => false
+
+def Res.getAssn? : Res → Option Assn
+| .sat assn => some assn
+| _         => none
+
+end Solver
+
+class Solver (m : Type → Type v) [outParam (Monad m)] where
+  solve : Formula → m Solver.Res
+
+namespace Solver
+
+class IpasirSolver (S : Type) (m : Type → Type v) [outParam (Monad m)] where
+  new : m S
+  addClause : Clause → S → m S
+  solve : S → m SolveRes
+
+instance [Monad m] [IpasirSolver S m] : Solver m where
+  solve f := do
+    let s : S ← IpasirSolver.new
+    let s ← f.clauses.foldlM (fun s c => IpasirSolver.addClause c s) s
+    IpasirSolver.solve s
+
+class ModelCount (m : Type → Type v) [outParam (Monad m)] where
+  modelCount : Formula → List Var → m Nat
+
+structure ApproxModelCount.Res where
+  mult : Nat
+  base : Nat
+  pow  : Nat
+deriving Inhabited
+
+instance : ToString ApproxModelCount.Res where
+  toString | ⟨mult,base,pow⟩ => s!"{mult} * {base}^{pow}"
+
+class ApproxModelCount (m : Type → Type v) [outParam (Monad m)] where
+  approxModelCount : Formula → List Var → m ApproxModelCount.Res
