LeanSAT/Solver/Dimacs.lean
@@ -1,0 +1,148 @@
+import LeanSAT.EncCNF
+import LeanSAT.Solver.Basic
+
+open Std
+
+namespace LeanSAT.Solver.Dimacs
+
+def formatVar : Var → String
+| (n : Nat) => s!"{n + 1}"
+
+def formatLit : Literal → String
+| .pos v => formatVar v
+| .neg v => "-" ++ formatVar v
+
+def formatClause : Clause → String
+| ⟨lits⟩ => lits.map (formatLit ·) ++ ["0"] |> String.intercalate " "
+
+def formatFormula (f : Formula) : String :=
+  let (vars,clauses) := (f.numVars, f.clauses.length)
+  s!"p cnf {vars} {clauses}\n" ++ (
+    f.clauses.map formatClause |> String.intercalate "\n" )
+
+def printFormula [Monad m] (print : String → m Unit) (f : Formula) : m Unit := do
+  let (vars,clauses) := (f.numVars, f.clauses.length)
+  print <| s!"p cnf {vars} {clauses}\n"
+  for c in f.clauses do
+    print <| formatClause c ++ "\n"
+
+example : (printFormula PrinterM.putStr ((0 ∨ 1) ∧ 5) |>.run) =
+"p cnf 6 2
+1 2 0
+6 0
+" := rfl
+
+def formatAssn (a : Assn) : String :=
+  a.fold (fun str v b =>
+    if b then
+      str.append s!" {v}"
+    else
+      str.append s!" -{v}")
+    "v"
+
+def printRes [Monad m] [MonadExcept ε m] [Inhabited ε] (print : String → m Unit) : Solver.Res → m Unit
+| .sat assn => do
+  print "s SATISFIABLE"
+  print (formatAssn assn)
+| .unsat => print "s UNSATISFIABLE"
+| .error => throw default
+
+
+def printEnc (s : EncCNF.State) : IO Unit := do
+  for i in [0:s.nextVar] do
+    for name in s.names.find? i do
+      IO.println s!"c {Dimacs.formatVar i} {name}"
+
+  Dimacs.printFormula IO.print ⟨s.clauses.reverse⟩
+
+
+
+
+
+structure DimacsParseRes where
+  vars : Nat
+  clauses : List Clause
+
+def parseVar (maxVar : Nat) (s : String) : Except String Var := do
+  let n ← s.toNat?.expectSome fun () => s!"Expected variable; got non-Nat: `{s}`"
+  match n with
+  | 0   => throw s!"Expected variable; got zero: `{s}`"
+  | v+1 =>
+    if v < maxVar then
+      return v
+    else
+      throw s!"Variable {v} higher than max var {maxVar}"
+
+def parseLit (maxVar : Nat) (s : String) : Except String Literal := do
+  if s.startsWith "-" then
+    parseVar maxVar (s.drop 1) |>.map Literal.not
+  else
+    parseVar maxVar s
+
+def parseClause (maxVar : Nat) (s : String) : Except String Clause := do
+  let lits ← s.splitOn " " |>.mapM (parseLit maxVar)
+  return ⟨lits⟩
+
+def parseHeader (s : String) : Except String (Nat × Nat) := do
+  match s.splitOn " " with
+  | ["p", "cnf", vars, clauses] => do
+    let vars ← vars.toNat?.expectSome     fun () => s!"Header line #vars: expected number, got `{vars}`"
+    let clss ← clauses.toNat?.expectSome  fun () => s!"Header line #clauses: expected number, got `{clauses}`"
+    return (vars, clss)
+  | _ => .error s!"Expected header `p cnf <#vars> <#clauses>`; got `{s}`"
+
+def parseFormula (s : String) : Except String DimacsParseRes := do
+  let ⟨pLine, clauseLines⟩ ←
+    s.splitOn "\n"
+    |>.filter (fun line => !line.startsWith "c" && line.any (!·.isWhitespace))
+    |>.expectNonempty fun () => "All lines are empty or comments"
+  let (nvars, _) ← parseHeader pLine
+  let clauses ← clauseLines.mapM (parseClause nvars)
+  return {
+    vars := nvars
+    clauses := clauses
+  }
+
+def parseAssnLine (maxVar : Var) (assn : Assn) (s : String) : Except String Assn := do
+  match ← (s.splitOn " " |>.expectNonempty fun () => panic! "splitOn returned empty?? 645") with
+  | ⟨"v", vars⟩ => do
+    let forAssn ← vars.foldlM (fun assn x => do
+      ForInStep.bind assn fun (assn : Assn) => do
+        if x = "0" then
+          return ForInStep.done assn
+        else
+          let l ← parseLit maxVar x
+          return ForInStep.yield <| assn.insertLit l
+    ) (ForInStep.yield assn)
+    return ForInStep.run forAssn
+  | _ =>
+    .error s!"Expected `v <lits>`, got `{s}`"
+
+def parseResult (maxVar : Var) (s : String) : Except String Solver.Res := do
+  let lines :=
+    s.splitOn "\n"
+    |>.filter (fun line => !line.startsWith "c" && line.any (!·.isWhitespace))
+  match ←(lines.expectNonempty fun () => s!"Expected result, got `{s}`") with
+  | ⟨first, rest⟩ =>
+  match first with
+  | "s UNSATISFIABLE" => return .unsat
+  | "s SATISFIABLE" =>
+    let assn ←
+      rest.foldlM (fun assn line => parseAssnLine maxVar assn line) (HashMap.empty)
+    return .sat assn
+  | _ => .error  "Expected `s <UNSATISFIABLE|SATISFIABLE>`, got `{first}`"
+
+
+def fromFileEnc (cnfFile : String) : IO EncCNF.State := do
+  let contents ← IO.FS.withFile cnfFile .read (·.readToEnd)
+  let {vars, clauses} ← IO.ofExcept <| Dimacs.parseFormula contents
+  return {
+    nextVar := vars
+    clauses := clauses
+    names := Id.run do
+      let mut map : HashMap Var String := HashMap.empty
+      for i in [0:vars] do
+        map := map.insert i s!"DIMACS var {i}"
+      return map
+    varCtx := ""
+  }
