LeanSAT/Solver/Impl/ApproxMCCommand.lean
@@ -1,0 +1,53 @@
+import LeanSAT.Solver.Basic
+import LeanSAT.Solver.Dimacs
+
+namespace LeanSAT.Solver.Impl
+
+
+/-- Command-line ApproxMC solver 
+
+Lives in IO, since we need access to process invocation.
+-/
+def ApproxMCCommand
+  (cmd : String := "approxmc") (flags : List String := []) : ApproxModelCount IO :=
+  ⟨fun fml sampleSet => do
+  let child ← IO.Process.spawn {
+    cmd := cmd
+    args := flags.toArray
+    stdin := .piped
+    stdout := .piped
+  }
+  let (stdin, child) ← child.takeStdin
+  stdin.putStrLn <| "c ind " ++ (sampleSet.map Dimacs.formatVar ++ ["0"] |> String.intercalate " ")
+  Dimacs.printFormula (stdin.putStr) fml
+  stdin.flush
+  let output ← IO.asTask child.stdout.readToEnd Task.Priority.dedicated
+  match ←child.wait with
+  | 0 =>
+    let outputStr ← IO.ofExcept output.get
+    IO.ofExcept <| parseOutput outputStr
+  | x =>
+    IO.ofExcept <| .error s!"Non-zero return code ({x}) from command: {cmd}"
+  ⟩
+where
+  parseOutput (s : String) : Except String ApproxModelCount.Res := do
+    let lines :=
+      s.splitOn "\n"
+      |>.filter (fun line => !line.startsWith "c" && line.any (!·.isWhitespace))
+    match lines with
+    | [] => .error s!"Expected outcome, got `{s}`"
+    | satRes :: rest =>
+    match satRes with
+    | "s UNSATISFIABLE" =>
+      return ⟨0,2,0⟩
+    | "s SATISFIABLE" =>
+      match rest with
+      | [] | _ :: _ :: _ =>
+        .error s!"Expected one content line after `s SATISFIABLE`, got `{rest}`"
+      | [res] =>
+      if !res.startsWith "s mc " then
+        .error s!"Expected `s mc <count>`, got `{s}`"
+      else
+      let number := res.drop 5 |>.trim
+      return ⟨← (number.toNat?.expectSome fun () => s!"Expected number, got {number}"), 2, 0⟩
+    | _ => .error s!"Expected `s [UN]SATISFIABLE`, got {satRes}"
