LeanSAT/Solver/Impl/DimacsCommand.lean
@@ -1,0 +1,34 @@
+import LeanSAT.Solver.Basic
+import LeanSAT.Solver.Dimacs
+
+
+namespace LeanSAT.Solver.Impl
+
+/-- Command-line DIMACS interface solver.
+
+This is the simplest solver to configure -- `cmd` is expected to
+be a command on the environment path which accepts DIMACS input
+and produces DIMACS output.
+
+This solver lives in IO, since we need access to process invocation.
+-/
+def DimacsCommand
+  (cmd : String) (flags : List String := []) : Solver IO :=
+  ⟨fun fml => do
+  IO.println "start"
+  let child ← IO.Process.spawn {
+    cmd := cmd
+    args := flags.toArray
+    stdin := .piped
+    stdout := .piped
+  }
+  let (stdin, child) ← child.takeStdin
+  IO.println "printing fml"
+  Dimacs.printFormula (stdin.putStr) fml
+  stdin.flush
+  IO.println "printed fml"
+  let output ← IO.asTask child.stdout.readToEnd Task.Priority.dedicated
+  let _ ← child.wait
+  let outputStr ← IO.ofExcept output.get
+  IO.ofExcept <| Dimacs.parseResult fml.numVars outputStr
+  ⟩
